AbsGraph.thy
@@ -1,0 +1,69 @@
+theory AbsGraph 
+imports GraalIR1_fromID
+begin
+
+(*
+datatype IRGraph =
+  Graph
+    (g_ids: "ID set")
+    (g_node: "ID \<Rightarrow> IRNode")
+    (g_inputs: "InputEdges")
+    (g_successors: "SuccessorEdges")
+*)
+definition empty_graph :: IRGraph where
+  "empty_graph =  (Graph {0} (\<lambda>i.(StartNode)) (\<lambda>i.[]) (\<lambda>i.[]))"
+
+lemma empty0 [simp]: "i \<in> g_ids empty_graph = (i = 0)"
+  unfolding empty_graph_def
+    by auto
+
+(* Get next free ID. *)
+fun next_id :: "IRGraph \<Rightarrow> nat" where
+  "next_id graph =  Max(g_ids graph) + 1"
+
+(* Get next n free IDs. *)
+fun next_ids :: "IRGraph \<Rightarrow> nat \<Rightarrow> nat list" where
+  "next_ids graph n = (let next = next_id graph in [next ..< next + n])"
+
+(* Extend a graph by adding one node to it. *)
+fun add_node :: "ID \<Rightarrow> IRNode \<Rightarrow> ID list \<Rightarrow> ID list \<Rightarrow> IRGraph \<Rightarrow> IRGraph" where
+  "add_node i node ins sucs g = (Graph
+      (g_ids g \<union> {i})
+      ((g_node g)(i := node))
+      ((g_inputs g)(i := ins))
+      ((g_successors g)(i := sucs))
+  )"
+
+(* Example 2:
+  public static int sq(int x) { return x * x; }
+
+             [1 P(0)]
+               \ /
+  [0 Start]   [4 *]
+       |      /
+       V     /
+      [5 Return]
+*)
+definition eg2_abs :: IRGraph where
+  "eg2_abs =
+    (add_node 5 ReturnNode [4] []
+    (add_node 4 MulNode [1, 1] []
+    (add_node 1 (ParameterNode 0) [] []
+    (add_node 0 StartNode [] [0]
+    empty_graph))))"
+
+lemma eg2node: "(g_node empty_graph)
+    (Suc 0 := ParameterNode 0,
+     4 := MulNode,
+     5 := ReturnNode) = eg2_node" 
+  unfolding fun_upd_apply
+  apply (simp only: fun_eq_iff)
+  unfolding empty_graph_def
+  apply auto
+  done
+
+lemma eq2: "eg2_abs = eg2_sq"
+  unfolding eg2_abs_def eg2_sq_def empty_graph_def
+  apply auto
+  
+end
